\documentclass{ctexart} % 中文友好
\usepackage{amsmath, amsthm, amssymb, graphicx, color}
\usepackage{geometry}
% 设置具体的边距
\geometry{a4paper, left=1cm, right=1cm, top=2.5cm, bottom=2.5cm}
\begin{document}
\section{累积量}
\[
F^{\left( k \right)}\left( s,t \right) =\left< \exp \left( se^{-i\varphi} \right) \right> ^{\left( k \right)}=\left< \sum_{m=0}^{\infty}{\frac{s^m}{m!}e^{-im\varphi}} \right> ^{\left( k \right)}\equiv \sum_{m=0}^{\infty}{{A_m}^{\left( k \right)}\left( t \right) \frac{s^m}{m!}}, {A_m}^{\left( k \right)}\left( t \right) =\frac{\partial ^m}{\partial s^m}\left. F^{\left( k \right)}\left( s,t \right) \right|_{s=0}
\]
\[
\#: \frac{\partial}{\partial t}F^{\left( k \right)}=-\left( i\omega _0+\gamma \right) s\frac{\partial}{\partial s}F^{\left( k \right)}-h_ks\frac{\partial ^2}{\partial s^2}F^{\left( k \right)}+{h_k}^*sF^{\left( k \right)}+r_{j\rightarrow k}\frac{p_j}{p_k}\left( F^{\left( j \right)}-F^{\left( k \right)} \right) .
\]
\[
\text{圆累积量：}\varPsi ^{\left( k \right)}\left( s,t \right) =s\frac{\partial}{\partial s}\ln F^{\left( k \right)}\left( s,t \right) \equiv \sum_{m=1}^{\infty}{{\varkappa _m}^{\left( k \right)}\left( t \right) s^m}, {\varkappa _m}^{\left( k \right)}\left( t \right) =\frac{1}{m!}\frac{\partial ^m}{\partial s^m}\left. \varPsi ^{\left( k \right)}\left( s,t \right) \right|_{s=0}.
\]
\[
\text{累积量：}\Phi ^{\left( k \right)}\left( s,t \right) \equiv \ln F^{\left( k \right)}\left( s,t \right) \equiv \sum_{m=1}^{\infty}{{K_m}^{\left( k \right)}\left( t \right) \frac{s^m}{m!}}, {K_m}^{\left( k \right)}\left( t \right) =\frac{\partial ^m}{\partial s^m}\left. \Phi ^{\left( k \right)}\left( s,t \right) \right|_{s=0}.
\]
\[
\text{简化记号：}F\Phi K_m\text{默认为}F^{\left( k \right)}\Phi ^{\left( k \right)}K_{m}^{\left( k \right)}\text{，}F^{\left( j \right)}\Phi ^{\left( j \right)}{K_m}^{\left( j \right)}\text{总是保留，}A=i\omega _0+\gamma , B=h_k, C={h_k}^*, D=r_{j\rightarrow k}\frac{m_j}{m_k},
\]
\[
\partial _tF=-As\partial _sF-Bs\partial _{s}^{2}F+CsF+D\left( F^{\left( j \right)}-F \right) ,
\]
\[
{\color[RGB]{192, 192, 192} F=\mathrm{e}^{\Phi}, \partial _sF=\mathrm{e}^{\Phi}\partial _s\Phi , \partial _{s}^{2}F=\mathrm{e}^{\Phi}\left( \left( \partial _s\Phi \right) ^2+\partial _{s}^{2}\Phi \right) ,}
\]
\[
{\color[RGB]{192, 192, 192} \partial _t\Phi =\frac{\partial _tF}{F}=-As\frac{\partial _sF}{F}-Bs\frac{{\partial ^2}_sF}{F}+Cs+D\left( \frac{F^{\left( j \right)}}{F}-1 \right) ,}
\]
\[
\#: \partial _t\Phi =-As\partial _s\Phi -Bs\left( \left( \partial _s\Phi \right) ^2+\partial _{s}^{2}\Phi \right) +Cs+D\left( e^{\Phi ^{\left( j \right)}-\Phi ^{\left( k \right)}}-1 \right) .
\]
\[
\Phi =\sum_{m=1}^{\infty}{K_m\frac{s^m}{m!}}=K_1s+K_2\frac{s^2}{2!}+K_3\frac{s^3}{3!}+\cdots , 
\]
\[
\Phi ^{\left( k \right)}=\sum_{m=1}^{\infty}{K_{m}^{\left( k \right)}\frac{s^m}{m!}}, \Phi ^{\left( j \right)}=\sum_{m=1}^{\infty}{K_{m}^{\left( j \right)}\frac{s^m}{m!}},
\]
\[
e^{\Phi ^{\left( j \right)}-\Phi ^{\left( k \right)}}=\sum_{m=0}^{\infty}{E_m\frac{s^m}{m!}},
\]
\[
1: \partial _t\Phi =\sum_{m=1}^{\infty}{\dot{K}_m\frac{s^m}{m!}}. {\color[RGB]{192, 192, 192} \partial _s\Phi =\sum_{m=1}^{\infty}{K_m\frac{s^{m-1}}{\left( m-1 \right) !}}=\sum_{n=0}^{\infty}{K_{n+1}\frac{s^n}{n!}}, }2: s\partial _s\Phi =\sum_{m=1}^{\infty}{mK_m\frac{s^m}{m!}}.
\]
\[
{\color[RGB]{192, 192, 192} \left( \sum_{n=0}^{\infty}{a_n\frac{s^n}{n!}} \right) \left( \sum_{n=0}^{\infty}{b_n\frac{s^n}{n!}} \right) =\sum\nolimits_{n=0}^{\infty}{c_n\frac{s^n}{n!},}\,\,\mathrm{where}}\ {\color[RGB]{128, 0, 0} c_n=\sum_{r=0}^n{\left( \begin{array}{c}
	n\\
	r\\
\end{array} \right) a_rb_{n-r}}}{\color[RGB]{192, 192, 192} ,}
\]
\[
{\color[RGB]{192, 192, 192} \left( \partial _s\Phi \right) ^2=\left( \sum_{n=0}^{\infty}{K_{n+1}\frac{s^n}{n!}} \right) \left( \sum_{n=0}^{\infty}{K_{n+1}\frac{s^n}{n!}} \right) =\sum_{n=0}^{\infty}{\left[ \sum_{r=0}^n{\left( \begin{array}{c}
	n\\
	r\\
\end{array} \right) K_{r+1}K_{n-r+1}} \right] \frac{s^n}{n!}},}
\]
\[
3\text{：} s\left( \partial _s\Phi \right) ^2=\sum_{m=1}^{\infty}{\left[ m\sum_{r=0}^{m-1}{\left( \begin{array}{c}
	m-1\\
	r\\
\end{array} \right) K_{r+1}K_{m-r}} \right] \frac{s^m}{m!}}.
\]
\[
4: s\partial _{s}^{2}\Phi ={\color[RGB]{192, 192, 192} s\sum_{m=2}^{\infty}{K_m\frac{s^{m-2}}{\left( m-2 \right) !}}=\sum_{n=2}^{\infty}{K_n\frac{s^{n-1}}{\left( n-2 \right) !}}=}\sum_{m=1}^{\infty}{mK_{m+1}\frac{s^m}{m!}}.
\]
\[
5: \mathrm{Complete} \mathrm{Bell} \mathrm{Polynomials}: 
\]
\[
\mathrm{Define} H=\Phi ^{\left( j \right) -}\Phi ^{\left( k \right)}=\sum_{m=1}^{\infty}{\Delta K_m\frac{s^m}{m!}}, \mathrm{e}^H=\sum_{m=0}^{\infty}{E_m\frac{s^m}{m!}}, 
\]
\[
\partial _s\mathrm{e}^H=H\prime \cdot \mathrm{e}^H, H\prime =\sum_{m=1}^{\infty}{\Delta K_m\frac{s^{m-1}}{\left( m-1 \right) !}}
\]
\[
H\prime \cdot \mathrm{e}^H=\left( \sum_{n=0}^{\infty}{\Delta K_{n+1}\frac{s^n}{n!}} \right) \left( \sum_{m=0}^{\infty}{E_m\frac{s^m}{m!}} \right) =\sum_{j=0}^{\infty}{\left( \sum_{k=0}^j{\left( \begin{array}{c}
	j\\
	k\\
\end{array} \right) \Delta K_{k+1}E_{j-k}} \right) \frac{s^j}{j!}},
\]
\[
\partial _s\mathrm{e}^H=\sum_{m=1}^{\infty}{E_m\frac{s^{m-1}}{\left( m-1 \right) !}}=\sum_{j=0}^{\infty}{E_{j+1}\frac{s^j}{j!}},
\]
\[
E_{j+1}=\sum_{k=0}^j{\left( \begin{array}{c}
	j\\
	k\\
\end{array} \right) \Delta K_{k+1}E_{j-k}}, j+1=m, r=m-1-k
\]
\[
E_m=\sum_{r=0}^{m-1}{\left( \begin{array}{c}
	m-1\\
	r\\
\end{array} \right) E_r}\cdot \Delta K_{m-r}, E_0=1,
\]
\[
\mathrm{e}^{\Phi ^{\left( j \right) -}\Phi ^{\left( k \right)}}-1 =\sum_{m=1}^{\infty}{E_m\frac{s^m}{m!}}.
\]
\\
\[
\#: 
\dot{K}_m=-mAK_m-mB\left[ \sum_{r=0}^{m-1}{\left( \begin{array}{c}
m-1\\
r\\
\end{array} \right) K_{r+1}K_{m-r}}+K_{m+1} \right] +C\delta _{m,1}+DE_m,
\]
\[
\mathrm{where}\ E_m=\sum_{r=0}^{m-1}{\left( \begin{array}{c}
m-1\\
r\\
\end{array} \right) E_r}\Delta K_{m-r},\ E_0=1,\ \Delta K_{m-r}=K_{m-r}^{\left( j \right)}-K_{m-r}^{\left( k \right)}.
\]
\[
\left\{ \begin{array}{c}
    \begin{array}{l}
    E_1=\Delta K_1,\\
    E_2=\Delta K_2+\left( \Delta K_1 \right) ^2,\\
    E_3=\Delta K_3+3\Delta K_1\Delta K_2+\left( \Delta K_1 \right) ^3\\
    \end{array}\\
    \cdots\\
\end{array} \right.
\]
\\
\[
\mathrm{Define}\ \kappa _m=\frac{K_m}{\left( m-1 \right) !}, 
\]
\[
\left( \begin{array}{c}
	m\\
	r\\
\end{array} \right) =\frac{m!}{r!\left( m-r \right) !}, \left( \begin{array}{c}
	m-1\\
	r\\
\end{array} \right) =\frac{\left( m-1 \right) !}{r!\left( m-1-r \right) !},
\]
\[
\,\,\kappa _{m-r}=\frac{K_{m-r}}{\left( m-r-1 \right) !}, E_m=\sum_{r=0}^{m-1}{\frac{E_r}{r!}\left( \kappa _{m-r}^{\left( j \right)}-\kappa _{m-r}^{\left( k \right)} \right)}
\]
\\
\[
\#:\dot{\kappa}_m=-mA\kappa _m-mB\left( \sum_{r=0}^{m-1}{\kappa _{r+1}\kappa _{m-r}}+m\kappa _{m+1} \right) +C\delta _{m,1}+DE_m,\\
\]
\[
\mathrm{where}\ E_m=\sum_{r=0}^{m-1}{\frac{E_r}{r!}\Delta \kappa _{m-r}}, \Delta \kappa _{m-r}=\kappa _{m-r}^{\left( j \right)}-\kappa _{m-r}^{\left( k \right)}, E_0=1.
\]
\[
\left\{ \begin{array}{c}
	\begin{array}{l}
	E_1=\Delta \kappa _1,\\
	E_2=\Delta \kappa _2+\left( \Delta \kappa _1 \right) ^2\\
	E_3=\Delta \kappa _3+\frac{2}{3}\Delta \kappa _1\Delta \kappa _2+\frac{1}{2}\left( \Delta \kappa _1 \right) ^3\\
\end{array}\\
	\cdots\\
\end{array} \right.
\]
\[
\mathcal{E} _m=\frac{E_m}{\left( m-1 \right) !}
\]
\[
\mathcal{E} _m\left( m-1 \right) !=\sum_{r=0}^{m-1}{\frac{\mathcal{E} _r}{r}\Delta \kappa _{m-r}}
\]
\end{document}